Refactoring MultiPaxos3.thy: separating the state of the acceptors and other things.

Isabelle2/MultiPaxos3.thy
@@ -1,6 +1,7 @@
 theory MultiPaxos3
 imports Main  "~~/src/HOL/Library/Monad_Syntax" "~~/src/HOL/Library/Code_Target_Nat"
   Log LinorderOption "~~/src/HOL/Library/FinFun_Syntax" "~~/src/HOL/Library/FSet"
+  "../../IO-Automata/IOA"
 begin
 
 text {* A version of MultiPaxos using FinFuns *}
@@ -36,7 +37,7 @@ type_synonym acc = nat
 
 datatype 'v msg =
   Phase1a (from_leader: acc) (ballot:bal)
-| Phase1b (last_votes:"nat \<Rightarrow>f ('v cmd \<times> bal) option") (new_ballot: bal) (acceptor:acc)
+| Phase1b (last_votes:"inst \<Rightarrow>f ('v cmd \<times> bal) option") (new_ballot: bal) (acceptor:acc)
 | Phase2a (inst: inst) (for_ballot:bal) (suggestion:"'v cmd") (leader: acc)
 | Phase2b (inst: inst) (ballot:bal) (acceptor: acc) (val: "'v cmd")
 | Vote (inst: inst) (val: "'v cmd")
@@ -48,38 +49,42 @@ datatype 'v  packet =
   -- {* A message with sender/destination information *}
   Packet (sender: acc) (dst: acc) (msg: "'v msg")
 
-record 'v mp_state =
+record 'v acc_state =
+  id :: acc
   acceptors :: "acc fset"
     -- {* The set of all acceptors *}
-  ballot :: "acc \<Rightarrow>f bal option"
+  ballot :: "bal option"
     -- {* the highest ballot in which an acceptor participated *}
-  vote :: "acc \<Rightarrow>f inst \<Rightarrow>f 'v cmd option"
+  vote :: "inst \<Rightarrow>f 'v cmd option"
     -- {* The last vote cast by an acceptor, for each instance *}
-  last_ballot :: "acc \<Rightarrow>f nat \<Rightarrow>f bal option"
+  last_ballot :: "nat \<Rightarrow>f bal option"
     -- {* For an acceptor a, this is the ballot in which "vote a" was cast, for each instance *}
-  onebs :: "acc \<Rightarrow>f bal \<Rightarrow>f inst \<Rightarrow>f (acc \<times> ('v cmd \<times> bal) option) list"
+  onebs :: "bal \<Rightarrow>f inst \<Rightarrow>f (acc \<times> ('v cmd \<times> bal) option) list"
     -- {* For an acceptor a and a ballot b, lists of 1b-message descriptions, indexed by ballot then instance. *}
-  twobs :: "acc \<Rightarrow>f inst \<Rightarrow>f bal \<Rightarrow>f acc list"
+  twobs :: "inst \<Rightarrow>f bal \<Rightarrow>f acc list"
     -- {* For an acceptor a: lists describing the 2b messages, indexed by instance then ballot. *}
-  decided :: "acc \<Rightarrow>f inst \<Rightarrow>f 'v cmd option"
-  next_inst :: "acc \<Rightarrow>f nat"
-  pending :: "acc \<Rightarrow>f inst \<Rightarrow>f 'v cmd option"
-  log :: "acc \<Rightarrow>f (nat \<times> 'v cmd) list"
-  leader :: "acc \<Rightarrow>f bool" (* TODO: we don't need the ballot here, because it's only used for the current ballot. *)
+  decided :: "inst \<Rightarrow>f 'v cmd option"
+  next_inst :: "nat"
+  pending :: "inst \<Rightarrow>f 'v cmd option"
+  leader :: "bool"
 
-definition init_state :: "acc fset \<Rightarrow> 'v mp_state" where
-  "init_state accs \<equiv> \<lparr>
-    mp_state.acceptors = accs,
-    ballot = K$ None,
-    vote = K$ K$ None,
-    last_ballot = K$ K$ None,
-    onebs = K$ K$ K$ [],
-    twobs = K$ K$ K$ [],
-    decided = K$ K$ None,
-    next_inst = K$ 1, (* instances start at 1 *)
-    pending = K$ K$ None,
-    log = K$ [],
-    leader = K$ False \<rparr>"
+fun accs where
+  "accs (0::nat) = {||}"
+| "accs (Suc n) = (accs n) |\<union>| {|Suc n|}"
+
+definition init_acc_state :: "nat \<Rightarrow> acc \<Rightarrow> 'v acc_state" where
+  "init_acc_state n a \<equiv> \<lparr>
+    id = a,
+    acc_state.acceptors = accs n,
+    ballot = None,
+    vote = K$ None,
+    last_ballot = K$ None,
+    onebs = K$ K$ [],
+    twobs = K$ K$ [],
+    decided = K$ None,
+    next_inst = 1, (* instances start at 1 *)
+    pending = K$ None,
+    leader = False \<rparr>"
 
 definition nr where
   -- {* The number of replicas *}
@@ -90,8 +95,8 @@ subsection {* Event handlers *}
 text {* If we had finfun_Ex we could do this better.
   Here we use instance 0 by default, but that's arbitrary. *}
 definition one_b_quorum_received where
-  "one_b_quorum_received a b s \<equiv> 
-    let at_b = onebs s $ a $ b;
+  "one_b_quorum_received b s \<equiv> 
+    let at_b = onebs s $ b;
         at_b_i = at_b $ 0
     in 2 * length at_b_i > nr s"
 
@@ -105,9 +110,10 @@ fun nx_bal where
 
 definition one_a_msgs where
   -- {* The set of 1a messages to send to try to become the leader *}
-  "one_a_msgs a s \<equiv> 
+  "one_a_msgs s \<equiv> 
     let
-      next_bal = nx_bal a (ballot s $ a) (nr s);
+      a = id s;
+      next_bal = nx_bal a (ballot s) (nr s);
       msg_1a = Phase1a a next_bal
     in {Packet a b msg_1a | b . b |\<in>| (acceptors s)}"
 
@@ -115,95 +121,67 @@ definition leader_of_bal where
   "leader_of_bal s b \<equiv> case b of None \<Rightarrow> 0 | Some b \<Rightarrow>
     (b mod (nr s))"
 
-definition send_all where "send_all s sendr m \<equiv> fimage (\<lambda> a2 . Packet sendr a2 m)  (acceptors s)"
+definition send_all where "send_all s m \<equiv> fimage (\<lambda> a2 . Packet (id s) a2 m)  (acceptors s)"
 
 definition do_2a where
-  "do_2a s a v \<equiv>
+  "do_2a s v \<equiv>
     let
-      inst = (next_inst s $ a);
-      msg = Phase2a inst (the (ballot s $ a)) v a;
-      new_state = s\<lparr>next_inst := (next_inst s)(a $:= inst+1),
-        pending := (pending s)(a $:= (pending s $ a)(inst $:= (Some v)))\<rparr>
+      a = id s;
+      inst = (next_inst s);
+      msg = Phase2a inst (the (ballot s)) v a;
+      new_state = s\<lparr>next_inst := (inst+1),
+        pending := (pending s)(inst $:= (Some v))\<rparr>
     in
-      (new_state, send_all s a msg)"
+      (new_state, send_all s msg)"
 
-definition propose :: "acc \<Rightarrow> 'v \<Rightarrow> 'v mp_state \<Rightarrow> ('v mp_state \<times> 'v packet fset)" where
+definition propose :: "'v \<Rightarrow> 'v acc_state \<Rightarrow> ('v acc_state \<times> 'v packet fset)" where
   -- {* If leader, then go ahead with 2a, otherwise forward to the leader. *}
-  "propose a v s \<equiv>
-    (if (leader_of_bal s (ballot s $ a) = a \<and> leader s $ a)
-      then do_2a s a (Cmd v)
-      else ( if (leader_of_bal s (ballot s $ a) = a)
+  "propose v s \<equiv> let a = id s in
+    (if (leader_of_bal s (ballot s) = a \<and> leader s)
+      then do_2a s (Cmd v)
+      else ( if (leader_of_bal s (ballot s) = a)
         then (s,{||}) (* TODO: here we loose the proposal... *)
-        else (s, {|Packet a (leader_of_bal s (ballot s $ a)) (Fwd (Cmd v))|})) )"
+        else (s, {|Packet a (leader_of_bal s (ballot s)) (Fwd (Cmd v))|})) )"
  
-fun receive_fwd where
-  "receive_fwd a (Fwd v) s = 
-    (if (leader_of_bal s (ballot s $ a) = a) then do_2a s a v else (s, ({||})))"
-| "receive_fwd a _ s = (s, ({||}))"
+definition receive_fwd  :: "'v \<Rightarrow> 'v acc_state \<Rightarrow> ('v acc_state \<times> 'v packet fset)" where
+  "receive_fwd v s \<equiv> let a = id s in 
+    (if (leader_of_bal s (ballot s) = a) then do_2a s (Cmd v) else (s, ({||})))"
 
-fun send_1a :: "acc \<Rightarrow> 'v mp_state \<Rightarrow> ('v mp_state \<times> 'v packet fset)" where
+definition send_1a :: "'v acc_state \<Rightarrow> ('v acc_state \<times> 'v packet fset)" where
   -- {* a tries to become the leader *}
-  "send_1a a s =
+  "send_1a s \<equiv>
     (let
-        b = nx_bal a (ballot s $ a) (nr s);
+        a = id s;
+        b = nx_bal a (ballot s) (nr s);
         msg_1a = Phase1a a b in
-      (s\<lparr>ballot := (ballot s)(a $:= Some b)\<rparr>, fimage (\<lambda> a2 . Packet a a2 msg_1a) (acceptors s)))"
+      (s\<lparr>ballot := Some b\<rparr>, fimage (\<lambda> a2 . Packet a a2 msg_1a) (acceptors s)))"
 
-export_code send_1a in Scala
-
-fun receive_1a :: "acc \<Rightarrow> 'v msg \<Rightarrow> 'v mp_state \<Rightarrow> ('v mp_state \<times> 'v packet fset)" where
-  "receive_1a a (Phase1a l b) s =
-    (let bal = ballot s $ a in
+definition receive_1a :: "acc \<Rightarrow> bal \<Rightarrow> 'v acc_state \<Rightarrow> ('v acc_state \<times> 'v packet fset)" where
+  "receive_1a l b s \<equiv>
+    (let bal = ballot s; a = id s in
       (if (bal = None \<or> ((the bal) < b))
        then
           (let
             combiner = (\<lambda> (vo,bo) . vo \<bind> (\<lambda> v . bo \<bind> (\<lambda> b . Some (v,b))));
-            last_votes = combiner o$ ($ vote s $ a, last_ballot s $ a $);
+            last_votes = combiner o$ ($ vote s, last_ballot s $);
             msg_1b = Phase1b last_votes b a;
             packet = Packet a l msg_1b;
-            state = s\<lparr>ballot := (ballot s)(a $:= Some b)\<rparr>
+            state = s\<lparr>ballot := Some b\<rparr>
           in
           (state, {|packet|}))
        else (s, {||})))"
-| "receive_1a a _ s = (s, {||})"
 
 definition update_onebs :: 
-  "'v mp_state \<Rightarrow> acc \<Rightarrow> bal \<Rightarrow> acc \<Rightarrow> (inst \<Rightarrow>f ('v cmd \<times> bal) option) \<Rightarrow> 'v mp_state" where
+  "'v acc_state \<Rightarrow> bal \<Rightarrow> acc \<Rightarrow> (inst \<Rightarrow>f ('v cmd \<times> bal) option) \<Rightarrow> 'v acc_state" where
   -- {* Update the list of highest voted values when receiving a 1b
     message from a2 for ballot bal containing last_vs *}
-  "update_onebs s a bal a2 last_vs \<equiv>
+  "update_onebs s bal a2 last_vs \<equiv>
     let
+      a = id s;
       combiner = \<lambda> (xs, y) . (case y of None \<Rightarrow> (a2, None)#xs | Some z \<Rightarrow> (a2, Some z)#xs);
-      pair_map = ($ (onebs s $ a $ bal), last_vs $);
+      pair_map = ($ (onebs s $ bal), last_vs $);
       at_bal = combiner o$ pair_map
-    in s\<lparr>onebs := (onebs s)(a $:= (onebs s $ a)(bal $:= at_bal))\<rparr>"
-
-abbreviation s1 where 
-  -- {* This is a state in which acceptor 1 is in ballot 2 and has received a ballot-2 1b message from
-  acceptor 2 saying that acceptor 2 last voted in ballot 1 in instance 1 for value 1. *}
-  "s1 \<equiv> \<lparr>
-    mp_state.acceptors = {|1,2,3|},
-    ballot = K$ Some 2,
-    vote = K$ K$ None,
-    last_ballot = K$ K$ None,
-    onebs = (K$ K$ K$ [])(1 $:= (K$ K$ [])(2 $:= (K$ [(2, None)])(1 $:= [(2, Some (Cmd 1,1))]))),
-    twobs = K$ K$ K$ [],
-    decided = K$ K$ None,
-    next_inst = K$ 1,
-    pending = K$ K$ None,
-    log = K$ [],
-    leader = K$ False \<rparr>"
-
-value "onebs test_state_1 $ 1 $ 2 $ 1"
-
-text {* State obtained after acceptor 1 receives a ballot-2 1b message from acceptor 3 saying that acceptor 3 never voted *}
-abbreviation s2 where "s2 \<equiv> update_onebs s1 1 2 3 (K$ None)"
-value "s2"
-value "onebs s2 $ 1 $ 2 $ 1"
-
-text {* State obtained after acceptor 1 receives a ballot-2 1b message from acceptor 3 saying that acceptor 3 last voted in instance 1 and ballot 1 for value 1 *}
-abbreviation s3 where  "s3 \<equiv> update_onebs s1 1 2 3 ((K$ None)(1 $:= Some (Cmd 1,1)))"
-value "onebs s3 $ 1 $ 2 $ 1"
+    in s\<lparr>onebs := (onebs s)(bal $:= at_bal)\<rparr>"
 
 definition highest_voted :: "(nat \<Rightarrow>f (acc \<times> ('v cmd \<times> nat) option) list) \<Rightarrow> (nat \<Rightarrow>f ('v cmd) option)" where
   -- {* Makes sense only if no list in the map is empty. *}
@@ -212,25 +190,6 @@ definition highest_voted :: "(nat \<Rightarrow>f (acc \<times> ('v cmd \<times> 
         votes = (map snd) o$ m;
         highest = (\<lambda> l . if (l = []) then None else (fold max l (l!0)) \<bind> (\<lambda> vb . Some (fst vb)))
     in highest o$ votes"
-
-text {* The highest n which has been updated (excluding updates to the default). 
-  The tentative below does not work.
-  Basically we would need to sort the domain and carry a sorted list in the result,
-  so that when we encounter a duplicate update then we can revise the max. *}
-
-abbreviation test :: "nat \<Rightarrow>f bool \<Rightarrow> (bool \<times> nat)"
-  where "test \<equiv> finfun_rec (\<lambda> (d::bool) . (d, 0)) 
-    (\<lambda> k v r . if (v \<noteq> fst r) 
-      then (fst r, max k (snd r)) else r)"
-
-interpretation finfun_rec_wf "(\<lambda> (d::bool) . (d, 0::nat))"
-  "(\<lambda> k v r . if (v \<noteq> fst r) then (fst r, max k (snd r)) else r)"
-apply(unfold_locales)
-apply auto[2]
-defer
-apply(simp split:split_if_asm)
-apply auto
-oops
 
 text {* Instead of trying to define the max as a recursive function, let's use finfun_to_list. *}
 value "((K$ False)(5 $:= True)(4 $:= False)(2 $:= True)) $ (2::int)"
@@ -246,138 +205,164 @@ text {*
 
   For now we propose values to all the instances ever started.
 *}
-fun receive_1b :: "acc \<Rightarrow> 'v msg \<Rightarrow> 'v mp_state \<Rightarrow> ('v mp_state \<times> 'v packet fset)" where
- "receive_1b a (Phase1b last_vs bal a2) s = (
-    if (Some bal = ballot s $ a)
+definition receive_1b :: "(inst \<Rightarrow>f ('v cmd \<times> bal) option) \<Rightarrow> bal \<Rightarrow> acc \<Rightarrow> 'v acc_state \<Rightarrow> ('v acc_state \<times> 'v packet fset)" where
+ "receive_1b last_vs bal a2 s \<equiv> (let a = id s in (
+    if (Some bal = ballot s)
     then
-      (let s1 = update_onebs s a bal a2 last_vs
-       in (if one_b_quorum_received a bal s1 
+      (let s1 = update_onebs s bal a2 last_vs
+       in (if one_b_quorum_received bal s1 
           then (let
-              h = highest_voted (onebs s1 $ a $ bal);
-              max_i = let l = (finfun_to_list (onebs s1 $ a $ bal)) in (if l = [] then 0 else hd (rev l));
-              s2 = s1\<lparr>leader := (leader s1)(a $:= True)\<rparr>;
-              s3 = s2\<lparr>next_inst := (next_inst s2)(a $:= max_i+1)\<rparr>;
+              h = highest_voted (onebs s1 $ bal);
+              max_i = let l = (finfun_to_list (onebs s1 $ bal)) in (if l = [] then 0 else hd (rev l));
+              s2 = s1\<lparr>leader := True\<rparr>;
+              s3 = s2\<lparr>next_inst := max_i+1\<rparr>;
               twoa_is = [1..<max_i+1];
               msgs = map (\<lambda> i . case h $ i of 
                   None \<Rightarrow> Phase2a i bal NoOp a
                 | Some v \<Rightarrow> Phase2a i bal v a) twoa_is;
-              pckts = map (\<lambda> m . send_all s a m) msgs
+              pckts = map (\<lambda> m . send_all s m) msgs
             in (s3, fold (op |\<union>|) pckts {||}) )
           else (s1, {||}) ) )
-    else (s, {||}))"
-| "receive_1b a _ s = (s, {||})"
+    else (s, {||})) )"
 
-fun receive_2a :: "acc \<Rightarrow> 'v msg \<Rightarrow> 'v mp_state \<Rightarrow> ('v mp_state \<times> 'v packet fset)" where
-  "receive_2a a (Phase2a i b v l) s =
-    (let bal = (ballot s $ a) in
+definition receive_2a :: "inst \<Rightarrow> bal \<Rightarrow> 'v cmd \<Rightarrow> acc \<Rightarrow> 'v acc_state \<Rightarrow> ('v acc_state \<times> 'v packet fset)" where
+  "receive_2a i b v l s =
+    (let a = id s; bal = (ballot s) in
       (if (bal = Some b)
-        then (s\<lparr>vote := (vote s)(a $:= (vote s $ a)(i $:= Some v))\<rparr>, send_all s a (Phase2b i b a v))
+        then (s\<lparr>vote := (vote s)(i $:= Some v)\<rparr>, send_all s (Phase2b i b a v))
         else (s, {||})))"
-| "receive_2a a _ s = (s, {||})"
 
-fun receive_2b :: "acc \<Rightarrow> 'v msg \<Rightarrow> 'v mp_state \<Rightarrow> ('v mp_state \<times> 'v packet fset)" where
-  "receive_2b a (Phase2b i b a2 v) s =
-    (if (decided s $ a $ i = None)
+definition receive_2b :: "inst \<Rightarrow> bal \<Rightarrow> acc \<Rightarrow> 'v cmd  \<Rightarrow> 'v acc_state \<Rightarrow> ('v acc_state \<times> 'v packet fset)" where
+  "receive_2b i b a2 v s \<equiv> let a = id s in 
+    (if (decided s $ i = None)
       then
         (let 
-            new_twobs = a2 # (twobs s $ a $ i $ b);
-            s2 = s\<lparr>twobs := (twobs s)(a $:= (twobs s $ a)(i $:= (twobs s $ a $ i)(b $:= new_twobs)))\<rparr>
+            new_twobs = a2 # (twobs s $ i $ b);
+            s2 = s\<lparr>twobs := (twobs s)(i $:= (twobs s $ i)(b $:= new_twobs))\<rparr>
         in
           (if (2 * length new_twobs > nr s)
-            then let
-                s3 = s2\<lparr>decided := (decided s2)(a $:= (decided s2 $ a)(i $:= Some v))\<rparr>;
-                s4 = s3\<lparr>log := (log s2)(a $:= distinct_Sorted_Insert (i, v) (log s $ a))\<rparr>
-              in
-                (s4, {||})
-            else
-              (s2, {||}) ) )
+            then (s2\<lparr>decided := (decided s2)(i $:= Some v)\<rparr>, {||})
+            else (s2, {||}) ) )
       else
         (s, {||}) )"
-| "receive_2b a _ s = (s, {||})"
-
-abbreviation s4 where 
-  -- {* This is a state in which acceptor 1 is in ballot 2 and has received a ballot-2 2b message from
-  acceptor 2 in instance 1. *}
-  "s4 \<equiv> \<lparr>
-    mp_state.acceptors = {|1,2,3|},
-    ballot = K$ Some 2,
-    vote = K$ K$ None,
-    last_ballot = K$ K$ None,
-    onebs = K$ K$ K$ [],
-    twobs = (K$ K$ K$ [])(1 $:= (K$ K$ [])(1 $:= (K$ [])(2 $:= [2]))),
-    decided = K$ K$ None,
-    next_inst = K$ 1,
-    pending = K$ K$ None,
-    log = K$ [],
-    leader = K$ False \<rparr>"
-
-text {* Acceptor 1 receives a round-2 2b message from acceptor 3 in instance 1. *}
-abbreviation step5 where "step5 \<equiv> receive_2b 1 (Phase2b 1 2 3 (Cmd (42::int))) s4"
-abbreviation s5 where "s5 \<equiv> fst step5"
-value "twobs s5 $ 1 $ 1 $ 2"
-value "decided s5 $ 1 $ 1"
-text {* Acceptor 1 receives a round-2 2b message from acceptor 1 in instance 1. *}
-abbreviation step6 where "step6 \<equiv> receive_2b 1 (Phase2b 1 2 1 (Cmd (42::int))) s5"
-abbreviation s6 where "s6 \<equiv> fst step6"
-text {* Since decided is already true, nothing is updated. *}
-value "twobs s6 $ 1 $ 1 $ 2"
 
 value "largestprefix [(1,v1), (2,v2), (4,v4)]"
 
-export_code send_1a receive_1a receive_1b init_state propose receive_2a receive_2b receive_fwd 
-  largestprefix in Scala file "simplePaxos.scala"
+text {* output transition could return an option *}
+definition learn :: "inst \<Rightarrow> 'v  \<Rightarrow> 'v acc_state \<Rightarrow> ('v acc_state \<times> 'v packet fset) option" where 
+  "learn i v s \<equiv> 
+    case (decided s $ i) of None \<Rightarrow> None |
+      Some cmd \<Rightarrow> (case cmd of NoOp \<Rightarrow> None 
+        | Cmd c \<Rightarrow> (if v = c then Some (s, {||}) else None))"
 
-subsection {* A test scenario*}
+export_code send_1a receive_1a receive_1b init_acc_state propose receive_2a receive_2b receive_fwd 
+  largestprefix learn in Scala file "simplePaxos.scala"
 
-text {* Process 1 acquires the leadership*}
-value "init_state {|1,2,3|}"
-abbreviation r1 where "r1 \<equiv> send_1a 1 (init_state {|1,2,3|})"
-abbreviation n1 where "n1 \<equiv> snd r1"
-value "fst r1"
-value "n1"
-abbreviation r2 where "r2 \<equiv> receive_1a 2 (Phase1a 1 4) (fst r1)"
-abbreviation n2 where "n2 \<equiv> n1 |\<union>| snd r2"
-value "fst r2"
-value "n2"
-abbreviation r3 where "r3 \<equiv> receive_1a 3 (Phase1a 1 4) (fst r2)"
-abbreviation n3 where "n3 \<equiv> n2 |\<union>| snd r3"
-value "fst r3"
-value "n3"
-abbreviation r4 where "r4 \<equiv> receive_1b 1 (Phase1b (K$ None) 4 2) (fst r3)"
-abbreviation n4 where "n4 \<equiv> n3 |\<union>| snd r4"
-value "fst r4"
-value "n4"
-abbreviation r5 where "r5 \<equiv> receive_1b 1 (Phase1b (K$ None) 4 3) (fst r4)"
-abbreviation n5 where "n5 \<equiv> n4 |\<union>| snd r5"
-value "highest_voted (onebs s1 $ 1 $ 4)"
-value "finfun_to_list (onebs s1 $ 1 $ 4)"
-value "one_b_quorum_received 1 4 (fst r5)"
-value "onebs (fst r5) $ 1 $ 4"
-value "fst r5"
-value "n5"
-text {* Now process 1 is the leader and proposes Cmd 1 *}
-abbreviation r6 where "r6 \<equiv> propose 1 (Cmd 1) (fst r5)"
-abbreviation n6 where "n6 \<equiv> snd r6" (* let's get rid of the previous messages to make things clearer *)
-value "fst r6"
-value "n6"
-abbreviation r7 where "r7 \<equiv> receive_2a 2 (Phase2a 1 4 (Cmd (Cmd 1)) 1) (fst r6)"
-abbreviation n7 where "n7 \<equiv> snd r7" (* let's get rid of the previous messages to make things clearer *)
-value "fst r7"
-value "n7"
-abbreviation r8 where "r8 \<equiv> receive_2a 3 (Phase2a 1 4 (Cmd (Cmd 1)) 1) (fst r7)"
-abbreviation n8 where "n8 \<equiv> snd r8 |\<union>| n7" 
-value "fst r8"
-value "n8"
-abbreviation r9 where "r9 \<equiv> receive_2b 1 (Phase2b 1 4 3 (Cmd (Cmd 1))) (fst r8)"
-abbreviation n9 where "n9 \<equiv> snd r9 |\<union>| n8" 
-value "fst r9"
-value "n9"
-text {* Upon receiving the second 2b message, process 1 decides Cmd 1 at position 1 *}
-abbreviation r10 where "r10 \<equiv> receive_2b 1 (Phase2b 1 4 2 (Cmd (Cmd 1))) (fst r9)"
-abbreviation n10 where "n10 \<equiv> snd r10 |\<union>| n9" 
-value "fst r10"
-value "n10"
-value "decided (fst r10) $ 1 $ 1"
-value "log (fst r10) $ 1"
+section {* The I/O-automata *}
+
+record 'v mp_state = 
+  node_states :: "nat \<Rightarrow>f 'v acc_state"
+  network :: "'v packet fset"
+
+datatype 'v mp_action =
+  Receive_fwd acc acc 'v
+| Propose acc 'v
+| Send_1as acc
+| Receive_1a_send_1b acc acc bal
+| Receive_1b acc acc "inst \<Rightarrow>f ('v cmd \<times> bal) option" bal
+| Receive_2a_send_2b acc acc inst bal "'v cmd"
+| Receive_2b acc acc inst bal "'v cmd"
+| Learn acc inst 'v
+
+locale mp_ioa = IOA +
+  fixes nas :: nat
+    -- {* The number of acceptors *}
+begin    
+
+definition mp_asig where
+  "mp_asig \<equiv>
+    \<lparr> inputs = { Propose a c | a c . a |\<in>| accs nas},
+      outputs = { Learn l i v | i v l . l |\<in>| accs nas},
+      internals = {Receive_fwd a1 a2 v | a1 a2 v . a1 |\<in>| accs nas \<and> a2 |\<in>| accs nas}
+        \<union> {Send_1as a | a . a |\<in>| accs nas}
+        \<union> {Receive_1a_send_1b a1 a2 b | a1 a2 b . a1 |\<in>| accs nas \<and> a2 |\<in>| accs nas}
+        \<union> {Receive_1b a1 a2 f b | a1 a2 f b . a1 |\<in>| accs nas \<and> a2 |\<in>| accs nas}
+        \<union> {Receive_2a_send_2b a1 a2 i b c | a1 a2 i b c . a1 |\<in>| accs nas \<and> a2 |\<in>| accs nas}
+        \<union> {Receive_2b a1 a2 i b c | a1 a2 i b c. a1 |\<in>| accs nas \<and> a2 |\<in>| accs nas}
+        \<union> {Learn a i c | a i c . a |\<in>| accs nas}\<rparr>"
+
+fun init_nodes_state where
+  "init_nodes_state (0::nat) n = undefined"
+| "init_nodes_state (Suc i) n = (init_nodes_state i n)(Suc i $:= init_acc_state n (Suc i))"
+
+lemma init_acc: 
+assumes "a \<le> n" and "a > 0"
+shows "(init_nodes_state a n) $ a = init_acc_state n a" using assms
+by (induct a n arbitrary:n rule:init_nodes_state.induct, auto)
+
+definition mp_start where
+  "mp_start \<equiv> {\<lparr>node_states = (init_nodes_state nas nas), network = {||}\<rparr>}"
+
+definition do_step :: "('v mp_state \<Rightarrow> ('v mp_state \<times> 'v packet set)) \<Rightarrow> 
+  (nat \<Rightarrow> 'v mp_state \<Rightarrow>'v mp_state \<Rightarrow> bool)" where 
+  "do_step step \<equiv> \<lambda> a s1 s2 . let (new_state, packets) =  (node_states gs1) in
+      gs2 = gs1\<lparr>node_states := new_state, network := (network gs1) |\<union>| packets\<rparr>"
+
+definition phase1_set1::"nat \<Rightarrow> 'v mp_state \<Rightarrow>'v mp_state \<Rightarrow> bool" where
+  "phase1_set1 l s s' \<equiv> (
+    let (new_state, packets) = send_1a l (node_states s) in
+      s' = s\<lparr>network := (network s) |\<union>| packets\<rparr>)"
+
+definition phase1_step2::"nat \<Rightarrow> 'v packet \<Rightarrow> 'v mp_state \<Rightarrow>'v mp_state \<Rightarrow> bool" where
+  "phase1_step2 acc p s s' \<equiv> 
+    dst p = acc \<and> p |\<in>| network s \<and>
+    (let (new_state, packets) = receive_1a acc (msg p) (node_states s) in
+      s' = s\<lparr>node_states := new_state, network := (network s) |\<union>| packets\<rparr>)"
+
+definition Receive1b::"nat \<Rightarrow> 'v packet \<Rightarrow> 'v mp_state \<Rightarrow>'v mp_state \<Rightarrow> bool" where
+  "Receive1b l p s s' \<equiv>
+    dst p = l \<and> p |\<in>| network s \<and>    
+    (let (new_state, packets) = receive_1b l (msg p) (node_states s) in
+      s' = s\<lparr>node_states := new_state, network := (network s) |\<union>| packets\<rparr>)"
+
+definition Send2a::"nat \<Rightarrow> 'v packet \<Rightarrow> 'v mp_state \<Rightarrow>'v mp_state \<Rightarrow> bool" where
+  "Send2a acc p s s' \<equiv> 
+    dst p = acc \<and> p \<in> network s \<and>
+    (let (new_state, packets) = receive_2a acc (msg p) (node_states s) in
+      s' = s\<lparr>node_states := new_state, network := (network s) \<union> packets\<rparr>)"
+
+definition Receive2b::"nat \<Rightarrow> 'v packet \<Rightarrow> 'v mp_state \<Rightarrow>'v mp_state \<Rightarrow> bool" where
+  "Receive2b l p s s' \<equiv>
+    dst p = l \<and> p \<in> network s \<and>    
+    (let (new_state, packets) = receive_2b l (msg p) (node_states s) in
+      s' = s\<lparr>node_states := new_state, network := (network s) \<union> packets\<rparr>)"
+
+definition ReceiveFwd::"nat \<Rightarrow> 'v packet \<Rightarrow> 'v mp_state \<Rightarrow>'v mp_state \<Rightarrow> bool" where
+  "ReceiveFwd acc p s s' \<equiv> 
+    dst p = acc \<and> p \<in> network s \<and>    
+    (let (new_state, packets) = receive_fwd acc (msg p) (node_states s) in
+      s' = s\<lparr>node_states := new_state, network := (network s) \<union> packets\<rparr>)"
+
+definition ProposeV::"nat \<Rightarrow> 'v \<Rightarrow> 'v mp_state \<Rightarrow>'v mp_state \<Rightarrow> bool" where
+  "ProposeV acc v s s' \<equiv>
+    (let (new_state, packets) = propose acc v (node_states s) in
+      s' = s\<lparr>node_states := new_state, network := (network s) \<union> packets\<rparr>)"
+
+fun p_trans_fun::"'v mp_state \<Rightarrow> 'v p_action \<Rightarrow> 'v mp_state \<Rightarrow> bool"  where
+  "p_trans_fun s (Send_1a l) s' = (Send1a l s s')"|
+  "p_trans_fun s (Respond_1a acc p) s' = (Receive1a acc p s s')"|
+  "p_trans_fun s (Respond_1b l p) s' = (Receive1b l p s s')"|
+  "p_trans_fun s (Send_2a acc p) s' = (Send2a acc p s s')"|
+  "p_trans_fun s (Respond_2b l p) s' = (Receive2b l p s s')"|
+  "p_trans_fun s (FwdA acc p) s' = (ReceiveFwd acc p s s')"|
+  "p_trans_fun s (Propose acc v) s' = (ProposeV acc v s s')"
+
+definition p_trans where
+  "p_trans \<equiv> { (r,a,r') . p_trans_fun r a r'}"
+
+definition p_ioa where
+  "p_ioa \<equiv> \<lparr>ioa.asig = p_asig, start = p_start, trans = p_trans\<rparr>"
+
+end
 
 end
